process and local type languages added  + lt2st relation

types/local.sig
@@ -1,0 +1,11 @@
+  local : Type
+  lpart : Type
+  llabel : Type
+  sort : Type
+  list : Functor
+  prod: Functor
+
+  ltend     : local
+  ltsend    : lpart -> "list" ("prod" ("prod" (llabel, sort), local)) -> local
+  ltreceive : lpart -> "list" ("prod" ("prod" (llabel, sort), local)) -> local
+  ltmu      : (local -> local) -> local
