src/st.v
@@ -4,73 +4,7 @@ Require Import ST.src.stream.
 Require Import String List.
 Local Open Scope string_scope.
 Import ListNotations.
-
-Notation label := string.
-Notation participant := string.
-
-Inductive sort: Type :=
-  | sunit: sort
-  | sbool: sort
-  | sint : sort
-  | snat : sort.
-
-Inductive subsort: sort -> sort -> Prop :=
-  | sni  : subsort snat sint
-  | srefl: forall s, subsort s s.
-
-Inductive nsubsort: sort -> sort -> Prop :=
-  | nsin: nsubsort sint snat
-  | nsbi: nsubsort sbool sint
-  | nsib: nsubsort sint sbool
-  | nsbn: nsubsort sbool snat
-  | nsnb: nsubsort snat sbool
-  | nsun: nsubsort sunit snat
-  | nsnu: nsubsort snat sunit
-  | nsbu: nsubsort sbool sunit
-  | nsub: nsubsort sunit sbool
-  | nsui: nsubsort sunit sint
-  | nsiu: nsubsort sint sunit.
-
-Lemma sort_dec: forall s s', subsort s s' \/ nsubsort s s'.
-Proof. intro s.
-       induction s; intros.
-       case_eq s'; intros.
-       left. apply srefl.
-       right. apply nsub.
-       right. apply nsui.
-       right. apply nsun.
-       case_eq s'; intros.
-       right. apply nsbu.
-       left. apply srefl.
-       right. apply nsbi.
-       right. apply nsbn.
-       case_eq s'; intros.
-       right. apply nsiu.
-       right. apply nsib.
-       left. apply srefl.
-       right. apply nsin.
-       case_eq s'; intros.
-       right. apply nsnu.
-       right. apply nsnb.
-       left. apply sni.
-       left. apply srefl.
-Qed.
-
-Lemma ssnssL: forall s t, subsort s t -> (nsubsort s t -> False).
-Proof. intro s.
-       induction s; intros; case_eq t; intros; subst; try easy.
-Qed.
-
-Lemma ssnssR: forall s t, nsubsort s t -> (subsort s t -> False).
-Proof. intro s.
-       induction s; intros; case_eq t; intros; subst; try easy.
-Qed.
-
-Class vector A n :=
-{
-  und : list A;
-  rest: length und = n
-}.
+Require Import ST.processes.process ST.types.local ST.processes.unscoped.
 
 
 (* session trees *)
@@ -78,12 +12,6 @@ CoInductive st: Type :=
   | st_end    : st
   | st_receive: participant -> list (label*sort*st) -> st
   | st_send   : participant -> list (label*sort*st) -> st.
-
-Fixpoint flattenT {A B C: Type} (l: list (A*B*C)): list C :=
-  match l with
-    | nil             => nil
-    | cons (a,b,c) xs => cons c (flattenT xs)
-  end.
 
 Inductive st_equiv (R: st -> st -> Prop): st -> st -> Prop :=
   | eq_st_end: st_equiv R st_end st_end
@@ -114,21 +42,16 @@ Definition st_id (s: st): st :=
 Lemma st_eq: forall s, s = st_id s.
 Proof. intro s; destruct s; easy. Defined.
 
-Lemma st_eq_inv: forall s t, s = t -> 
-  (s = st_end /\ t = st_end) \/
-  (exists p p' l l', s = st_receive p l /\ t = st_receive p' l' /\ p = p' /\ l' = l') \/
-  (exists p p' l l', s = st_send p l /\ t = st_send p' l' /\ p = p' /\ l' = l').
-Proof. intros.
-       destruct s; destruct t.
-       left. easy.
-       easy.
-       easy.
-       easy.
-       right. left.
-       exists s. exists s0. exists l. exists l0. inversion H. easy.
-       easy. easy. easy.
-       right. right.
-       exists s. exists s0. exists l. exists l0. inversion H. easy.
-Qed.
+Inductive lt2st (R: local -> st -> Prop): local -> st -> Prop :=
+  | lt2st_end: lt2st R lt_end st_end
+  | lt2st_rcv: forall p l s xs ys,
+               List.Forall (fun u => R (fst u) (snd u)) (zip xs ys) ->
+               lt2st R (lt_receive p (zip (zip l s) xs)) (st_receive p (zip (zip l s) ys))
+  | lt2st_snd: forall p l s xs ys,
+               List.Forall (fun u => R (fst u) (snd u)) (zip xs ys) ->
+               lt2st R (lt_send p (zip (zip l s) xs)) (st_send p (zip (zip l s) ys))
+  | lt2st_mu : forall l t,
+               lt2st R (l [lt_mu l .: lt_var]) t ->
+               lt2st R (lt_mu l) t.
 
-
+Definition lt2stC l t := paco2 lt2st bot2 l t.
