completeness/completeness.v
@@ -1,5 +1,5 @@
-Require Import ST.src.stream ST.src.st ST.src.so ST.src.si 
-               ST.src.reordering ST.src.siso 
+Require Import ST.src.stream ST.processes.process ST.src.st ST.src.so ST.src.si 
+               ST.src.reordering ST.src.siso ST.types.local
                ST.subtyping.refinement ST.src.reorderingfacts ST.subtyping.subtyping 
                ST.negations.nrefinement ST.negations.nsubtyping.
 Require Import Coq.Logic.Classical_Pred_Type Coq.Logic.ClassicalFacts Coq.Logic.Classical_Prop.
