examples/Example4_14.v
@@ -1,4 +1,5 @@
-Require Import ST.src.stream ST.src.st ST.src.so ST.src.si ST.src.reordering ST.src.siso ST.subtyping.refinement ST.src.reorderingfacts ST.subtyping.subtyping.
+Require Import ST.src.stream ST.processes.process ST.src.st ST.src.so ST.src.si ST.src.reordering ST.src.siso ST.types.local
+               ST.subtyping.refinement ST.src.reorderingfacts ST.subtyping.subtyping.
 From mathcomp Require Import all_ssreflect seq ssrnat.
 From Paco Require Import paco.
 Require Import String List Coq.Arith.Even.
