negations/nrefinement.v
@@ -1,5 +1,5 @@
-Require Import ST.src.stream ST.src.st ST.src.so ST.src.si 
-               ST.src.reordering ST.src.siso 
+Require Import ST.src.stream ST.processes.process ST.src.st ST.src.so ST.src.si 
+               ST.src.reordering ST.src.siso ST.types.local
                ST.subtyping.refinement ST.src.reorderingfacts.
 From mathcomp Require Import all_ssreflect seq.
 From Paco Require Import paco.
